README.md
@@ -7,17 +7,10 @@ C_0 := 0, ~ C_{n+1} := \sum_{i=0}^{n} C_i C_{n-i}
 $$
 
 ## Instructions
-Create a Lean project that uses `mathlib` as a dependency by running the command:
-```bash
-lake +leanprover-community/mathlib4:lean-toolchain new catalan-numbers math
-```
-`cd` into the newly created `catalan-numbers` folder and run the command:
+Clone the project, `cd` into it and configure `mathlib` by running the command:
 ```bash
 lake exe cache get
 ```
-Then you can clone this repo and place the file `catalan_numbers.lean`into the
-`CatalanNumbers` folder of the `catalan-numbers` project. The entire project is 
-contained in this file.
 
 ## Troubleshooting
 - For mathlib related issues, look at [this](https://github.com/leanprover-community/mathlib4/wiki/Using-mathlib4-as-a-dependency)
